Made State inductive

DataTypes.v
@@ -1,5 +1,4 @@
 Module Type DataTypes.
-
   Parameter classical: forall P, P \/ ~ P.
 
   Parameter Addr: Set.
@@ -10,7 +9,109 @@ Module Type DataTypes.
   Definition Index := nat.
 
   Parameter parent: Cache -> Cache.
-  Definition State := nat.
+  Inductive State := In | Sh | Ow | Mo.
+
+  Definition slt x y := match x with
+                          | In => match y with
+                                    | In => False
+                                    | Sh => True
+                                    | Ow => True
+                                    | Mo => True
+                                  end
+                          | Sh => match y with
+                                    | In => False
+                                    | Sh => False
+                                    | Ow => True
+                                    | Mo => True
+                                  end
+                          | Ow => match y with
+                                    | In => False
+                                    | Sh => False
+                                    | Ow => False
+                                    | Mo => True
+                                  end
+                          | Mo => False
+                        end.
+  Definition sgt x y := slt y x.
+  Definition sle x y := match x with
+                          | In => match y with
+                                    | In => True
+                                    | Sh => True
+                                    | Ow => True
+                                    | Mo => True
+                                  end
+                          | Sh => match y with
+                                    | In => False
+                                    | Sh => True
+                                    | Ow => True
+                                    | Mo => True
+                                  end
+                          | Ow => match y with
+                                    | In => False
+                                    | Sh => False
+                                    | Ow => True
+                                    | Mo => True
+                                  end
+                          | Mo => match y with
+                                    | In => False
+                                    | Sh => False
+                                    | Ow => False
+                                    | Mo => True
+                                  end
+                        end.
+
+  Theorem sle_eq: forall {x y}, x = y -> sle x y.
+  Proof.
+    intros x y x_eq_y. rewrite x_eq_y.
+    unfold sle.
+    destruct y; auto.
+  Qed.
+
+  Theorem slt_neq: forall {x y}, x = y -> ~ slt x y.
+  Proof.
+    intros x y x_eq_y. rewrite x_eq_y. intros geez.
+    unfold slt in geez.
+    destruct y; auto.
+  Qed.
+
+  Theorem slt_neq': forall {x y}, slt x y -> x <> y.
+  Proof.
+    unfold slt; destruct x; destruct y; auto; discriminate.
+  Qed.
+
+  Theorem slt_slti_false: forall {x y}, slt x y -> slt y x -> False.
+  Proof.
+    intros x y slt1 slt2.
+    unfold slt in *; destruct x in *; destruct y in *; auto.
+  Qed.
+
+  Theorem slt_slei_false: forall {x y}, slt x y -> sle y x -> False.
+  Proof.
+    intros x y s1 s2.
+    unfold slt in *; unfold sle in *; destruct x in *; destruct y in *; auto.
+  Qed.
+
+  Theorem not_slt_sle: forall {x y}, ~ slt x y -> sle y x.
+  Proof.
+    intros x y noSlt.
+    unfold sle; unfold slt in *;
+    destruct x; destruct y; auto.
+  Qed.
+
+  Theorem slt_eq_slt_dec: forall {x y}, slt x y \/ x = y \/ slt y x.
+  Proof.
+    intros x y.
+    destruct x; destruct y; unfold slt; auto.
+  Qed.
+
+  Theorem slt_eq_sle: forall {x y}, sle x y = slt x y \/ x = y.
+  Proof.
+    intros x y.
+    unfold sle; unfold slt.
+    destruct x; destruct y; auto.
+  Qed.
+    
+
   Definition Time := nat.
   Parameter state: Cache -> Addr -> Time -> State.
   Parameter dir: Cache -> Cache -> Addr -> Time -> State.
@@ -27,11 +128,4 @@ Module Type DataTypes.
   Parameter Label : Set.
   Inductive StLabel := Initial | Store : Label -> StLabel.
   Parameter data: Cache -> Addr -> Time -> StLabel.
-
-  Definition Mo := 3.
-  Definition Ow := 2.
-  Definition Sh := 1.
-  Definition In := 0.
-  Parameter maxState: forall {c a t}, state c a t <= Mo.
-  Parameter maxDir: forall {p c a t}, parent c = p -> dir p c a t <= Mo.
 End DataTypes.
